cedar-dafny/pe/interpretation.dfy
@@ -1,0 +1,93 @@
+include "../def/core.dfy"
+include "../def/base.dfy"
+include "../difftest/main.dfy"
+include "../def/std.dfy"
+include "def.dfy"
+
+module pe.interpretation {
+  import opened def.core
+  import opened def.base
+  import difftest.restrictedExpr
+  import opened def.std
+  import opened definition
+
+  datatype Interpretation = Interpretation(mappings: string -> core.Expr) {
+    ghost predicate wellFormed() {
+      forall v :: restrictedExpr.evaluate(mappings(v)).Some?
+    }
+
+    function interpret(r: Residual): definition.Result<core.Value>
+      requires wellFormed()
+    {
+      match r {
+        case Concrete(v) => Ok(v)
+        case If(c, t, e) => Err(TypeError)
+        case Unknown(u: Unknown) => Ok(restrictedExpr.evaluate(mappings(u.name)).value)
+        case _ => Err(TypeError)
+      }
+    }
+
+    function replaceUnknownInOptionalEntity(oe: OptionalEntity): (r: Option<core.EntityUID>)
+      requires wellFormed()
+    {
+      match oe {
+        case Left(l) => Some(l)
+        case Right(u) =>
+          var v := restrictedExpr.evaluate(mappings(u.name)).value;
+          if v.Primitive? && v.primitive.EntityUID? then
+            Some(v.primitive.uid)
+          else
+            None
+      }
+    }
+
+    function replaceRecord(context: definition.Record): Option<core.Record>
+      requires wellFormed() {
+      var nr := map a: Attr | a in context.Keys :: interpret(context[a]);
+      if forall a | a in nr.Keys :: nr[a].Ok? then
+        Some(map a | a in nr.Keys :: nr[a].value)
+      else
+        None
+    }
+
+    function replaceUnknownInRequest(req: definition.Request): Option<core.Request>
+      requires wellFormed()
+    {
+      var p :- replaceUnknownInOptionalEntity(req.principal);
+      var a :- replaceUnknownInOptionalEntity(req.action);
+      var r :- replaceUnknownInOptionalEntity(req.resource);
+      var c :- replaceRecord(req.context);
+      Some(core.Request(p, a, r, c))
+    }
+
+    function replaceUnknownInEntityStore(store: definition.EntityStore): Option<core.EntityStore>
+      requires wellFormed() {
+      var entities := map euid: EntityUID | euid in store.entities.Keys :: match replaceRecord(store.entities[euid].attrs) {
+                                                                             case Some(r) => Some(core.EntityData(r, store.entities[euid].ancestors))
+                                                                             case None => None
+                                                                           };
+      if forall euid | euid in entities.Keys :: entities[euid].Some? then
+        Some(core.EntityStore(map euid | euid in entities.Keys :: entities[euid].value))
+      else
+        None
+    }
+
+    function replaceUnknownInExpr(e: definition.Expr): core.Expr {
+      match e {
+        case PrimitiveLit(p) => core.PrimitiveLit(p)
+        case Var(v) => core.Var(v)
+        case If(c, t, else_e) => core.If(replaceUnknownInExpr(c), replaceUnknownInExpr(t), replaceUnknownInExpr(else_e))
+        case And(e1, e2) => core.And(replaceUnknownInExpr(e1), replaceUnknownInExpr(e2))
+        case Or(e1, e2) => core.Or(replaceUnknownInExpr(e1), replaceUnknownInExpr(e2))
+        case UnaryApp(o, op_e) => core.UnaryApp(o, replaceUnknownInExpr(op_e))
+        case BinaryApp(o, e1, e2) => core.BinaryApp(o, replaceUnknownInExpr(e1), replaceUnknownInExpr(e2))
+        case GetAttr(entity_e, a) => core.GetAttr(replaceUnknownInExpr(entity_e), a)
+        case HasAttr(entity_e, a) => core.HasAttr(replaceUnknownInExpr(entity_e), a)
+        case Set(es) => core.Expr.Set(seq(|es|, i requires 0 <= i < |es| => replaceUnknownInExpr(es[i])))
+        case Record(bs) => core.Expr.Record(seq(|bs|, i requires 0 <= i < |bs| => (bs[i].0, replaceUnknownInExpr(bs[i].1))))
+        case Call(name, args) => core.Call(name, seq(|args|, i requires 0 <= i < |args| => replaceUnknownInExpr(args[i])))
+        case Unknown(u) => mappings(u.name)
+      }
+    }
+  }
+}
