cedar-dafny/pe/soundness.dfy
@@ -1,0 +1,21 @@
+include "def.dfy"
+include "interpretation.dfy"
+include "engine.dfy"
+include "../def/core.dfy"
+include "../def/engine.dfy"
+
+module pe.soundness {
+  import opened definition
+  import opened interpretation
+  import opened engine
+  import ce = def.engine
+  import def.core
+
+  lemma PEIsSound(e: definition.Expr, q: core.Request, s: core.EntityStore, Q: definition.Request, S: definition.EntityStore, I: Interpretation)
+    requires I.wellFormed()
+    requires var pr := I.replaceUnknownInRequest(Q); pr.Some? && pr.value == q
+    requires var ps := I.replaceUnknownInEntityStore(S); ps.Some? && ps.value == s
+    ensures var peRes := PartialEvaluator(Q, S).interpret(e);
+            (peRes.Ok? ==> ce.Evaluator(q, s).interpret(I.replaceUnknownInExpr(e)) == I.interpret(peRes.value)) &&
+            (peRes.Err? ==> ce.Evaluator(q, s).interpret(I.replaceUnknownInExpr(e)).Err?)
+}
